theories/Compositional_Structures/Basic_Modules/Elect_Module_Ref.thy
@@ -6,15 +6,21 @@ begin
 
  \<comment> \<open>The elect module should not return just the reference to all alternatives
   but a deep copy\<close>
+
+
+
+
+
 fun elect_module_ref :: "'a Electoral_Module_Ref" where
-  "elect_module_ref A p =
-   FOREACH A
-     (\<lambda> x (e,r,d). RETURN ((insert x e), r, d)) ({},{},{})"
+  "elect_module_ref A p = do {
+   B <- aux_set_copy A;
+   RETURN (B,{},{})
+}"
 
 lemma elect_module_ref_correct:
   shows "(elect_module_ref, (\<lambda> A p. SPEC (\<lambda> res. res= elect_module A p)))
       \<in> elec_mod_relb"
-  unfolding elect_module_ref.simps elect_module.simps
+  unfolding elect_module_ref.simps elect_module.simps aux_set_copy_def
   apply (intro fun_relI)
 proof (rename_tac A' A pl pr)
   fix A' A:: "'a set"
@@ -22,22 +28,27 @@ proof (rename_tac A' A pl pr)
   assume arel: "(A', A) \<in> \<langle>Id\<rangle>alt_set_rel"
   from arel have aeq: "A' = A" by (auto simp add: alt_set_rel_def in_br_conv)
   from arel have fina: "finite A" by (auto simp add: alt_set_rel_def in_br_conv)
-  have "(FOREACH A' (\<lambda>x (e, r, d). RETURN (insert x e, r, d)) ({}, {}, {}),
+  from fina have refid: "(FOREACH A' (\<lambda>x cp. RETURN (insert x cp)) {} \<bind> (\<lambda>B. RETURN (B, {}, {})),
         SPEC (\<lambda>res. res = (A, {}, {})))
        \<in> \<langle>Id\<rangle>nres_rel"
-  apply (refine_vcg FOREACH_rule[where I = "\<lambda>it (e,r,d). e = A' - it \<and> r = {} \<and> d = {}"])
-    by (auto simp add: aeq fina)
-  from this show "(FOREACH A' (\<lambda>x (e, r, d). RETURN (insert x e, r, d)) ({}, {}, {}),
+    apply (refine_vcg)
+    apply (simp add: aeq)
+    using aux_set_copy_correct aux_set_copy_def
+    by (metis singleton_conv)
+    show "(FOREACH A' (\<lambda>x cp. RETURN (insert x cp)) {} \<bind> (\<lambda>B. RETURN (B, {}, {})),
         SPEC (\<lambda>res. res = (A, {}, {})))
        \<in> \<langle>\<langle>Id\<rangle>set_rel \<times>\<^sub>r \<langle>Id\<rangle>set_rel \<times>\<^sub>r \<langle>Id\<rangle>set_rel\<rangle>nres_rel"
+      apply (refine_vcg)
+    using refid[THEN nres_relD] prod_rel_id set_rel_id
     by simp
 qed
+
   
 
 sepref_definition elect_sepref is 
   "uncurry elect_module_ref" :: "(alts_set_impl_assn)\<^sup>k *\<^sub>a (profile_impl_assn)\<^sup>k
     \<rightarrow>\<^sub>a (result_impl_assn)"
-  unfolding elect_module_ref.simps
+  unfolding elect_module_ref.simps aux_set_copy_def
   apply (rewrite in "\<hole>" hs.fold_custom_empty)+
   by sepref
 
